split the ordered context stuff out into its own file

theories/Reflection/OExpr_untyped.v
@@ -1,503 +1,10 @@
 Require Export PredMonad.Reflection.OrderedType.
+Require Export PredMonad.Reflection.OrderedContext.
 Require Import Coq.Logic.ProofIrrelevance.
 
 Import EqNotations.
 Import ListNotations.
 Import ProofIrrelevanceTheory.
-
-(***
- *** Pairs of Types + Relations
- ***)
-
-(* Shorthand for type + relation *)
-Notation "'TpRel'" := (sigT OTRelation).
-
-(* Shorthand for building type + relation pairs *)
-Notation "'mkTpRel' A" := (existT OTRelation A _)
-                            (left associativity, at level 20).
-
-(* Shorthand for equalities on types + relations *)
-Notation "A =t= B" := (existT OTRelation A%type _ = existT OTRelation B%type _)
-                        (no associativity, at level 70).
-
-(* OTRelation instance for the first projection of a type + relation pair *)
-Instance OTRelation_projT1 (tprel:TpRel) : OTRelation (projT1 tprel) :=
-  projT2 tprel.
-
-(* A pfun that converts from an otype to an equal one *)
-Definition eq_pfun A B {RA:OTRelation A} {RB:OTRelation B} (e:A =t= B) :
-  A -o> B :=
-  match e in _ = existT _ B _ with
-  | eq_refl => id_pfun
-  end.
-Arguments eq_pfun {_ _ _ _} !e.
-
-(* Composing two eq_pfuns composes the equality proofs *)
-Lemma compose_eq_pfun {A B C}
-      {RA:OTRelation A} {RB:OTRelation B} {RC:OTRelation C}
-      (e1:A =t= B) (e2:B =t= C) (e3:A =t= C) :
-  compose_pfun (eq_pfun e1) (eq_pfun e2) =o= eq_pfun e3.
-Proof.
-  assert (A =t= B) as e1'; [ assumption | ].
-  assert (B =t= C) as e2'; [ assumption | ].
-  revert e1 e2 e3; dependent rewrite e1'; dependent rewrite e2'; intros.
-  repeat (rewrite (UIP_refl _ _ _); simpl).
-  split; intros c1 c2 Rc; apply Rc.
-Qed.
-
-(* An eq_pfun on two equal types simplifies to the identity *)
-Lemma eq_pfun_refl {A} {RA:OTRelation A} (e:A =t= A) : eq_pfun e = id_pfun.
-Proof.
-  rewrite (UIP_refl _ _ e). reflexivity.
-Qed.
-
-Lemma eqTpTupleR {A B C} {RA:OTRelation A} {RB:OTRelation B} {RC:OTRelation C} :
-  A =t= B -> A*C =t= B*C.
-Proof.
-  intro e; dependent rewrite e; reflexivity.
-Defined.
-
-(* commute eq_pfun before a pfun_curry inside it *)
-Lemma commute_eq_curry_pfun {A1 A2 B C}
-      `{OType A1} `{OType A2} `{OTRelation B} `{OTRelation C}
-      (e:A1 =t= A2) (f : (A2 * B) -o> C) :
-  compose_pfun (eq_pfun e) (pfun_curry f) =o=
-  pfun_curry (compose_pfun (eq_pfun (eqTpTupleR e)) f).
-Proof.
-  assert (A1 =t= A2) as e'; try assumption.
-  revert H e f; dependent rewrite e'; intros.
-  rewrite (UIP_refl _ _ e). simpl.
-  split; intros x1 x2 Rx y1 y2 Ry; simpl; apply pfun_Proper; split; assumption.
-Qed.
-
-(* commute eq_pfun inside a pfun_apply *)
-Lemma commute_eq_apply_pfun {A1 A2 B C}
-      `{OTRelation A1} `{OTRelation A2} `{OTRelation B} `{OTRelation C}
-      (e:A1 =t= A2) (f: A2 -o> B -o> C) g :
-  compose_pfun (eq_pfun e) (pfun_apply f g) =o=
-  pfun_apply (compose_pfun (eq_pfun e) f) (compose_pfun (eq_pfun e) g).
-Proof.
-  assert (A1 =t= A2) as e'; try assumption.
-  revert e f g; dependent rewrite e'; intros. rewrite (UIP_refl _ _ _). simpl.
-  split; intros x1 x2 Rx; simpl;
-    assert (f @o@ x1 <o= f @o@ x2) as Rfx;
-    try (apply pfun_Proper; assumption);
-    apply Rfx; apply pfun_Proper; assumption.
-Qed.
-
-Lemma eq_pfun_adjoint_l {A1 A2 B}
-      `{OTRelation A1} `{OTRelation A2} `{OTRelation B}
-      (e12:A1 =t= A2) (e21:A2 =t= A1) f g :
-  compose_pfun (eq_pfun e12) f =o= g <-> f =o= compose_pfun (eq_pfun e21) g.
-Proof.
-  assert (A1 =t= A2) as e'; try assumption.
-  revert f g e12 e21; dependent rewrite <- e'; intros.
-  rewrite (UIP_refl _ _ e12); rewrite (UIP_refl _ _ e21); simpl.
-  split; intros [Rfg Rgf]; split; intros x y Rxy; simpl;
-    first [ apply Rfg | apply Rgf ]; assumption.
-Qed.
-
-Lemma eq_pfun_adjoint_r {A1 A2 B}
-      `{OTRelation A1} `{OTRelation A2} `{OTRelation B}
-      (e12:A1 =t= A2) (e21:A2 =t= A1) f g :
-  compose_pfun f (eq_pfun e12) =o= g <-> f =o= compose_pfun g (eq_pfun e21).
-Proof.
-  assert (A1 =t= A2) as e'; try assumption.
-  revert f g e12 e21; dependent rewrite <- e'; intros.
-  rewrite (UIP_refl _ _ e12); rewrite (UIP_refl _ _ e21); simpl.
-  split; intros [Rfg Rgf]; split; intros x y Rxy; simpl;
-    first [ apply Rfg | apply Rgf ]; assumption.
-Qed.
-
-
-(***
- *** Ordered Type Contexts
- ***)
-
-(* A context here is just a list of types *)
-Inductive Ctx : Type :=
-| CtxNil
-| CtxCons A `{OTRelation A} (ctx:Ctx)
-.
-
-(* An element of a context is a nested tuple of elements of its types *)
-Fixpoint CtxElem (ctx:Ctx) : Type :=
-  match ctx with
-  | CtxNil => unit
-  | CtxCons A ctx' => CtxElem ctx' * A
-  end.
-
-(* OTRelation instance for any CtxElem type *)
-Instance OTRelation_CtxElem ctx : OTRelation (CtxElem ctx).
-Proof.
-  induction ctx.
-  - apply OTunit_R.
-  - apply OTpair_R; assumption.
-Defined.
-
-(* A context is valid iff each ordered type in it is valid *)
-Fixpoint ValidCtxF ctx : Prop :=
-  match ctx with
-  | CtxNil => True
-  | CtxCons A ctx' =>
-    OType A /\ ValidCtxF ctx'
-  end.
-
-(* Typeclass version of ValidCtxF *)
-Class ValidCtx ctx : Prop := validCtx : ValidCtxF ctx.
-
-(* Instances for building ValidCtx proofs *)
-Instance ValidCtx_Nil : ValidCtx CtxNil := I.
-Instance ValidCtx_Cons A `{OType A} ctx (vc:ValidCtx ctx) :
-  ValidCtx (CtxCons A ctx) := conj _ vc.
-
-(* OType instance of CtxElem of a valid context *)
-Instance OType_CtxElem ctx (valid:ValidCtx ctx) : OType (CtxElem ctx).
-Proof.
-  induction ctx; [ | destruct valid ]; typeclasses eauto.
-Qed.
-
-(* Convert an equality on context to one on CtxElems *)
-Definition eqCtxElem {ctx1 ctx2} (e:ctx1=ctx2) :
-  (CtxElem ctx1) =t= (CtxElem ctx2) :=
-  match e in _ = ctx2 with
-  | eq_refl => eq_refl
-  end.
-
-(* Helper pfun that converts between equal contexts *)
-Definition eq_ctx_pfun {ctx1 ctx2} e : CtxElem ctx1 -o> CtxElem ctx2 :=
-  eq_pfun (eqCtxElem e).
-Arguments eq_ctx_pfun {_ _ } e /.
-
-(* Get the head type of a context, defaulting to unit *)
-Definition ctxHead ctx : Type :=
-  match ctx with
-  | CtxNil => unit
-  | CtxCons A _ => A
-  end.
-
-Instance OTRelation_ctxHead ctx : OTRelation (ctxHead ctx) :=
-  match ctx with
-  | CtxNil => _
-  | CtxCons _ _ => _
-  end.
-
-Instance OType_ctxHead ctx `{valid:ValidCtx ctx} : OType (ctxHead ctx).
-Proof.
-  destruct ctx.
-  - typeclasses eauto.
-  - exact (proj1 valid).
-Qed.
-
-(* Get the tail of a context, defaulting to the empty context *)
-Definition ctxTail ctx :=
-  match ctx with
-  | CtxNil => CtxNil
-  | CtxCons _ ctx' => ctx'
-  end.
-
-Instance ValidCtx_ctxTail ctx `{valid:ValidCtx ctx} : ValidCtx (ctxTail ctx).
-Proof.
-  destruct ctx.
-  - typeclasses eauto.
-  - exact (proj2 valid).
-Qed.
-
-(* Non-nil contexts equal cons of their heads and tails *)
-Lemma ctx_eq_head_tail ctx :
-  ctx <> CtxNil -> ctx = CtxCons (ctxHead ctx) (ctxTail ctx).
-  destruct ctx; intro e.
-  elimtype False; apply e; reflexivity.
-  reflexivity.
-Qed.
-
-(* Look up the nth type in a Ctx, returning the unit type as a default *)
-Fixpoint ctxNth n ctx {struct ctx} : Type :=
-  match ctx with
-  | CtxNil => unit
-  | CtxCons A ctx' =>
-    match n with
-    | 0 => A
-    | S n' => ctxNth n' ctx'
-    end
-  end.
-Arguments ctxNth !n !ctx.
-
-(* The OTRelation for the nth type in a context *)
-Instance OTRelation_ctxNth n ctx : OTRelation (ctxNth n ctx).
-Proof.
-  revert n; induction ctx; intros; simpl; try typeclasses eauto.
-  destruct n; simpl; typeclasses eauto.
-Defined.
-Arguments OTRelation_ctxNth !n !ctx.
-
-(* For valid contexts, the nth element is a valid OType *)
-Instance OType_ctxNth n ctx `{valid:ValidCtx ctx} : OType (ctxNth n ctx).
-Proof.
-  revert n valid; induction ctx; intros; simpl; try typeclasses eauto.
-  destruct valid. destruct n; try assumption. apply IHctx; apply H1.
-Qed.
-
-(* The ctxNth of nil is always unit *)
-Lemma ctxNth_nil n : ctxNth n CtxNil =t= unit.
-Proof.
-  induction n; reflexivity.
-Qed.
-
-(* Pfun to extract the nth element of a context *)
-Fixpoint nth_pfun ctx n : CtxElem ctx -o> ctxNth n ctx :=
-  match ctx return CtxElem ctx -o> ctxNth n ctx with
-  | CtxNil => const_pfun tt
-  | CtxCons A ctx' =>
-    match n return CtxElem (CtxCons A ctx') -o> ctxNth n (CtxCons A ctx') with
-    | 0 => snd_pfun
-    | S n' => compose_pfun fst_pfun (nth_pfun ctx' n')
-    end
-  end.
-Arguments nth_pfun !ctx !n.
-
-(* Appending contexts *)
-(* FIXME: is this needed? *)
-Fixpoint appendCtx ctx1 ctx2 : Ctx :=
-  match ctx1 with
-  | CtxNil => ctx2
-  | CtxCons A ctx1' =>
-    CtxCons A (appendCtx ctx1' ctx2)
-  end.
-
-(* Context length *)
-(* FIXME: is this needed? *)
-Fixpoint ctxLen ctx :=
-  match ctx with
-  | CtxNil => 0
-  | CtxCons A ctx' => S (ctxLen ctx')
-  end.
-
-
-(***
- *** Context Insertion, aka Weakening
- ***)
-
-(* Weaken a context by inserting a type at point w *)
-Fixpoint ctxInsert w W {RW:OTRelation W} ctx : Ctx :=
-  match w with
-  | 0 => CtxCons W ctx
-  | S w' =>
-    match ctx with
-    | CtxNil => CtxCons unit (ctxInsert w' W CtxNil)
-    | CtxCons B ctx' => CtxCons B (ctxInsert w' W ctx')
-    end
-  end.
-Arguments ctxInsert !w W {RW} !ctx.
-
-(* A context is valid iff its weakening with a valid OType is *)
-Lemma ValidCtx_ctxInsert_iff n W `{OType W} ctx :
-  ValidCtx ctx <-> ValidCtx (ctxInsert n W ctx).
-Proof.
-  split; revert ctx; induction n; intro ctx; destruct ctx; simpl; intro valid;
-    repeat (lazymatch goal with | |- _ /\ _ => split | _ => idtac end);
-    repeat (lazymatch goal with | H:_ /\ _ |- _ => destruct H | _ => idtac end);
-    try typeclasses eauto; apply I.
-Qed.
-
-(* Weakening preserves validity *)
-Instance ValidCtx_insert w W `{OType W} ctx {valid:ValidCtx ctx} :
-  ValidCtx (ctxInsert w W ctx).
-Proof.
-  apply ValidCtx_ctxInsert_iff; assumption.
-Qed.
-
-(* ctxInsert commutes with ctxTail by incrementing the weakening position *)
-Lemma ctxInsert_ctxTail n A {RA:OTRelation A} ctx :
-  ctxInsert n A (ctxTail ctx) = ctxTail (ctxInsert (S n) A ctx).
-Proof.
-  revert ctx; induction n; intros; destruct ctx; reflexivity.
-Qed.
-
-(* The head of a weakened context at non-zero position is just the head of the
-original context *)
-Lemma ctxHead_ctxInsert_S n A {RA:OTRelation A} ctx :
-  ctxHead (ctxInsert (S n) A ctx) =t= ctxHead ctx.
-Proof.
-  destruct ctx; reflexivity.
-Qed.
-
-(* Map from a weaker to a stronger context, by dropping the new element *)
-Fixpoint weaken_pfun w W {RW:OTRelation W} ctx :
-  CtxElem (ctxInsert w W ctx) -o> CtxElem ctx :=
-  match w return CtxElem (ctxInsert w W ctx) -o> CtxElem ctx with
-  | 0 => fst_pfun (H:=OTRelation_CtxElem _)
-  | S w' =>
-    match ctx return CtxElem (ctxInsert (S w') W ctx) -o> CtxElem ctx with
-    | CtxNil => const_pfun tt
-    | CtxCons B ctx' =>
-      pair_pfun (compose_pfun fst_pfun (weaken_pfun w' W ctx')) snd_pfun
-    end
-  end.
-Arguments weaken_pfun !w W {RW} !ctx.
-
-(* Weaken an index in a context, to make ctxNth commute with ctxInsert *)
-Fixpoint weakenIndex w (n:nat) {struct w} : nat :=
-  match w with
-  | 0 => S n
-  | S w' =>
-    match n with
-    | 0 => 0
-    | S n' => S (weakenIndex w' n')
-    end
-  end.
-Arguments weakenIndex !w !n.
-
-(* Weakening commutes with ctxNth *)
-Lemma weaken_ctxNth w W {RW:OTRelation W} ctx n :
-  ctxNth (weakenIndex w n) (ctxInsert w W ctx) =t= ctxNth n ctx.
-Proof.
-  revert ctx n; induction w; intros; destruct ctx; simpl.
-  - reflexivity.
-  - reflexivity.
-  - destruct n; simpl; try reflexivity. rewrite <- (ctxNth_nil n). apply IHw.
-  - destruct n; simpl; try reflexivity. apply IHw.
-Qed.
-
-(* FIXME: put this somewhere more appropriate *)
-Lemma unit_eq_tt (x:unit) : x =o= tt.
-Proof.
-  destruct x; reflexivity.
-Qed.
-
-(* FIXME: put this somewhere more appropriate *)
-Definition pfun_unit_eq_tt {A} {RA:OTRelation A} (f g: A -o> unit) : f =o= g.
-  (* FIXME: why doesn't unit_eq_tt work without an arg on both sides? *)
-  split; intros x y Rxy; repeat rewrite (unit_eq_tt (_ @o@ _));
-    reflexivity.
-Qed.
-
-(* Weakening followed by nth is just the extended nth *)
-Lemma weaken_nth_pfun w W `{OType W} ctx {valid:ValidCtx ctx} n :
-  compose_pfun (weaken_pfun w W ctx) (nth_pfun ctx n)
-  =o= compose_pfun (nth_pfun (ctxInsert w W ctx) (weakenIndex w n))
-                   (eq_pfun (weaken_ctxNth w W ctx n)).
-Proof.
-  revert ctx valid n; induction w; intros; destruct ctx; destruct n; simpl;
-    try apply pfun_unit_eq_tt; destruct valid.
-  - rewrite eq_pfun_refl. rewrite compose_id_pfun. reflexivity.
-  - rewrite eq_pfun_refl. rewrite compose_id_pfun. reflexivity.
-  - rewrite eq_pfun_refl. rewrite compose_pair_snd.
-    rewrite compose_id_pfun. reflexivity.
-  - rewrite compose_compose_pfun. rewrite compose_pair_fst.
-    rewrite <- compose_compose_pfun. rewrite IHw; try assumption.
-    rewrite compose_compose_pfun. f_equiv. f_equiv. apply proof_irrelevance.
-Qed.
-
-
-(***
- *** Context Deletion, aka Substitution
- ***)
-
-(* Delete the nth element of a context *)
-Fixpoint ctxDelete n ctx {struct ctx} : Ctx :=
-  match ctx with
-  | CtxNil => CtxNil
-  | CtxCons A ctx' =>
-    match n with
-    | 0 => ctx'
-    | S n' => CtxCons A (ctxDelete n' ctx')
-    end
-  end.
-Arguments ctxDelete !n !ctx.
-
-Instance ValidCtx_ctxDelete n ctx {valid:ValidCtx ctx} :
-  ValidCtx (ctxDelete n ctx).
-Proof.
-  revert n valid; induction ctx; intros n valid;
-    [ | destruct n; destruct valid ]; simpl.
-  - apply I.
-  - assumption.
-  - split; [ | apply IHctx ]; assumption.
-Qed.
-
-(* The the n+1-th suffix of a context *)
-Fixpoint ctxSuffix n ctx {struct ctx} : Ctx :=
-  match ctx with
-  | CtxNil => CtxNil
-  | CtxCons A ctx' =>
-    match n with
-    | 0 => ctx'
-    | S n' => ctxSuffix n' ctx'
-    end
-  end.
-
-Instance ValidCtx_ctxSuffix n ctx {valid:ValidCtx ctx} :
-  ValidCtx (ctxSuffix n ctx).
-Proof.
-  revert n valid; induction ctx; intros n valid;
-    [ | destruct n; destruct valid ]; simpl.
-  - apply I.
-  - assumption.
-  - apply IHctx; assumption.
-Qed.
-
-Fixpoint subst_pfun ctx n :
-  (CtxElem (ctxSuffix n ctx) -o> ctxNth n ctx) ->
-  CtxElem (ctxDelete n ctx) -o> CtxElem ctx :=
-  match ctx return
-        (CtxElem (ctxSuffix n ctx) -o> ctxNth n ctx) ->
-        CtxElem (ctxDelete n ctx) -o> CtxElem ctx with
-  | CtxNil => fun s => const_pfun tt
-  | CtxCons A ctx' =>
-    match n return
-        (CtxElem (ctxSuffix n (CtxCons A ctx')) -o> ctxNth n (CtxCons A ctx')) ->
-        CtxElem (ctxDelete n (CtxCons A ctx')) -o> CtxElem (CtxCons A ctx')
-    with
-    | 0 => fun s => pair_pfun id_pfun s
-    | S n' =>
-      fun s =>
-        pair_pfun (compose_pfun fst_pfun (subst_pfun ctx' n' s)) snd_pfun
-    end
-  end.
-
-(* Helper shortcut for the repeated types in subst_var_pfun *)
-Definition subst_var_tp ctx n v :=
-  (CtxElem (ctxSuffix n ctx) -o> ctxNth n ctx) ->
-  CtxElem (ctxDelete n ctx) -o> ctxNth v ctx.
-
-(* Substitute into a variable v, which may or may not equal n *)
-Fixpoint subst_var_pfun ctx n v {struct ctx} :
-  (CtxElem (ctxSuffix n ctx) -o> ctxNth n ctx) ->
-  CtxElem (ctxDelete n ctx) -o> ctxNth v ctx :=
-  match ctx return subst_var_tp ctx n v with
-  | CtxNil => fun s => const_pfun tt
-  | CtxCons A ctx' =>
-    match n return subst_var_tp (CtxCons A ctx') n v with
-    | 0 =>
-      match v return subst_var_tp (CtxCons A ctx') 0 v with
-      | 0 => fun s => s
-      | S v' => fun _ => nth_pfun ctx' v'
-      end
-    | S n' =>
-      match v return subst_var_tp (CtxCons A ctx') (S n') v with
-      | 0 => fun _ => snd_pfun
-      | S v' =>
-        fun s => compose_pfun fst_pfun (subst_var_pfun ctx' n' v' s)
-      end
-    end
-  end.
-
-Lemma subst_nth_pfun ctx n v s {valid:ValidCtx ctx} :
-  compose_pfun (subst_pfun ctx n s) (nth_pfun ctx v) =o=
-  subst_var_pfun ctx n v s.
-Proof.
-  revert n v s valid; induction ctx; intros;
-    [ | destruct n; destruct v; destruct valid ]; simpl.
-  - rewrite compose_const_pfun_f. reflexivity.
-  - apply compose_pair_snd.
-  - rewrite compose_compose_pfun. rewrite compose_pair_fst.
-    rewrite id_compose_pfun. reflexivity.
-  - apply compose_pair_snd.
-  - rewrite compose_compose_pfun. rewrite compose_pair_fst.
-    rewrite <- compose_compose_pfun. f_equiv. apply IHctx. assumption.
-Qed.
-
 
 (***
  *** Ordered Expressions
@@ -1006,11 +513,12 @@ Fixpoint substOVar n (s:OExpr) vctx v : OExpr :=
     end
   | S n' =>
     match v with
-    | 0 => OVar (ctxDelete n' (ctxTail vctx)) 0
+    | 0 => OVar (ctxDelete (S n') vctx) 0
     | S v' =>
       weakenOExpr 0 (ctxHead vctx) (substOVar n' s (ctxTail vctx) v')
     end
   end.
+Arguments substOVar !n s vctx !v.
 
 (* Substitution for ordered expressions *)
 Fixpoint substOExpr n (s:OExpr) (e:OExpr) : OExpr :=
@@ -1021,6 +529,47 @@ Fixpoint substOExpr n (s:OExpr) (e:OExpr) : OExpr :=
   | OLam body => OLam (substOExpr (S n) s body)
   end.
 
+
+FIXME HERE NOW: need an equivalence on contexts, basically saying that
+ctxNth is the same for all indices (so, e.g., CtxNil equiv cons of all units)
+
+Lemma HasType_substOVar n s vctx v {valid:ValidCtx vctx} :
+  HasType (ctxSuffix n vctx) (ctxNth n vctx) s ->
+  HasType (ctxDelete n vctx) (ctxNth v vctx) (substOVar n s vctx v).
+Proof.
+  revert n vctx valid v; induction n; intros; destruct v.
+  - destruct vctx; assumption.
+  - destruct vctx; simpl; split; try split; try reflexivity.
+    destruct valid; assumption.
+  - destruct vctx; simpl; split; try split; try reflexivity.
+    + destruct valid; assumption.
+    + apply ValidCtx_ctxDelete; destruct valid; assumption.
+  - destruct vctx; simpl.
+
+Lemma substOExpr_HasType n s e ctx A {RA:OTRelation A} :
+  HasType (ctxSuffix n ctx) (ctxNth n ctx) s -> HasType ctx A e ->
+  HasType (ctxDelete n ctx) A (substOExpr n s e).
+Admitted.
+
+Lemma var_substitution n s vctx v
+      (ht: HasTypeC (ctxDelete n vctx) (ctxNth v vctx) (substOVar n s vctx v))
+      (ht_s: HasTypeC (ctxSuffix n vctx) (ctxNth n vctx) s) :
+  exprSemantics (ctxDelete n vctx) _ (substOVar n s vctx v) ht =o=
+  subst_var_pfun vctx n v (exprSemantics _ _ s ht_s).
+Admitted.
+
+Lemma substitution n s e ctx A {RA:OTRelation A}
+      (ht: HasTypeC ctx A e)
+      (ht_s: HasTypeC (ctxSuffix n ctx) (ctxNth n ctx) s)
+      (ht_subst: HasTypeC (ctxDelete n ctx) A (substOExpr n s e)) :
+  exprSemantics (ctxDelete n ctx) A (substOExpr n s e) ht_subst =o=
+  compose_pfun (subst_pfun ctx n (exprSemantics _ _ s ht_s))
+               (exprSemantics ctx A e ht).
+Admitted.
+
+Theorem OExpr_beta B {RB:OTRelation B} e1 e2 :
+  oexpr_eq (OApp B (OLam e1) e2) (substOExpr 0 e2 e1).
+Admitted.
 
 FIXME HERE NOW: prove correctness of substitution!
 
